theories/Combined.v
@@ -516,7 +516,7 @@ Section Simulation.
     }
     assert (¬ safe (#() #()) (<[ℓ := #0]> σ)) as Hnotsafe.
     {
-      apply stuck_not_safe, head_stuck_stuck, ectxi_language_sub_redexes_are_values.
+      apply stuck_not_safe, base_stuck_stuck, ectxi_language_sub_redexes_are_values.
       - split ; first done. inversion 1.
       - intros [] ; try discriminate 1 ; inversion 1 ; by eauto.
     }
@@ -669,7 +669,7 @@ Section Soundness.
       (* — either e = Var x: *)
       + (* then Var x is stuck *)
         exfalso. eapply stuck_not_safe; [|done]. rewrite translation_fill.
-        apply stuck_fill, head_stuck_stuck.
+        apply stuck_fill, base_stuck_stuck.
         { split; [done|]. intros ???? Hstep. inversion Hstep. }
         apply ectxi_language_sub_redexes_are_values=>-[] //.
       (* — either e = K[Fork e1]: *)
